proof/invariants/findBlockInKS.v
@@ -336,10 +336,9 @@ intro kernelstructurestart.
 	unfold isPDT in *.
 	destruct (lookup idPD (memory s) beqAddr) eqn:Hlookup ; try (exfalso ; congruence).
 	destruct v eqn:Hv ; try (exfalso ; congruence).
-	unfold consistency in *.
-	unfold StructurePointerIsKS in *. intuition.
+	assert(HSPIsKS : StructurePointerIsKS s) by (unfold consistency in * ; intuition).
 	subst.
-	apply H16 with idPD. assumption.
+	apply HSPIsKS with idPD. assumption.
 }
 Qed.
 
@@ -371,10 +370,9 @@ intro kernelstructurestart.
 	unfold isPDT in *.
 	destruct (lookup idPD (memory s) beqAddr) eqn:Hlookup ; try (exfalso ; congruence).
 	destruct v eqn:Hv ; try (exfalso ; congruence).
-	unfold consistency in *.
-	unfold StructurePointerIsKS in *. intuition.
+	assert(HSPIsKS : StructurePointerIsKS s) by (unfold consistency in * ; intuition).
 	subst.
-	apply H15 with idPD. assumption.
+	apply HSPIsKS with idPD. assumption.
 }
 Qed.
 
